start to convert to a datatype

lib/Marshalling/MarshalledAccessors.i.dfy
@@ -6,51 +6,60 @@ module MarshalledAccessors {
   import opened NativePackedInts
   import opened Sequences
 
-  method Uint32ArrayLength(data: seq<byte>, start: uint64) returns (length: uint64)
-    requires |data| < Uint64UpperBound()
-    requires start as int <= |data|
-    requires parse_Uint32Array(data[start..]).0.Some?
-    ensures length as int == |parse_Uint32Array(data[start..]).0.value.va|
+  datatype MarshalledUint32Array = MarshalledUint32Array(data: seq<byte>, start: uint64)
   {
-    length := Unpack_LittleEndian_Uint64(data[start..], 0);
-  }
+    predicate WF() {
+      && |data| < Uint64UpperBound()
+      && start as int <= |data|
+      && parse_Uint32Array(data[start..]).0.Some?
+    }
 
-  method Uint32ArraySize(data: seq<byte>, start: uint64) returns (size: uint64)
-    requires |data| < Uint64UpperBound()
-    requires start as int <= |data|
-    requires parse_Uint32Array(data[start..]).0.Some?
-    ensures size as int == SizeOfV(parse_Uint32Array(data[start..]).0.value)
-  {
-    var length := Uint32ArrayLength(data, start);
-    size := 8 + 4 * length;
-  }
+    function I() : seq<uint32>
+      requires WF()
+    {
+      parse_Uint32Array(data[start..]).0.value.va
+    }
   
-  method Uint32ArrayElement(data: seq<byte>, start: uint64, i: uint64) returns (element: uint32)
-    requires |data| < Uint64UpperBound()
-    requires start as int <= |data|
-    requires parse_Uint32Array(data[start..]).0.Some?
-    requires i as int < |parse_Uint32Array(data[start..]).0.value.va|
-    ensures element == parse_Uint32Array(data[start..]).0.value.va[i]
-  {
-    var idx := 8 + i * 4;
-    element := Unpack_LittleEndian_Uint32(data, start + idx);
+    method Length() returns (length: uint64)
+    requires WF()
+    ensures length as int == |I()|
+    {
+      length := Unpack_LittleEndian_Uint64(data[start..], 0);
+    }
 
-    ghost var len := |parse_Uint32Array(data[start..]).0.value.va|;
+    method Size() returns (size: uint64)
+      requires WF()
+      ensures size as int == SizeOfV(VUint32Array(I()))
+    {
+      var length := Length();
+      size := 8 + 4 * length;
+    }
+  
+    method Element(i: uint64) returns (element: uint32)
+      requires WF()
+      requires i as int < |I()|
+      ensures element == I()[i]
+    {
+      var idx := 8 + i * 4;
+      element := Unpack_LittleEndian_Uint32(data, start + idx);
+
+      ghost var len := |parse_Uint32Array(data[start..]).0.value.va|;
     
-    calc {
-      element;
-      unpack_LittleEndian_Uint32(data[start + idx..start + idx + 4]);
-      { lemma_seq_suffix_slice(data, start as int, idx as int, idx as int + 4); }
-      unpack_LittleEndian_Uint32(data[start..][idx..idx + 4]);
-      unpack_LittleEndian_Uint32(data[start..][8 + i * 4..8 + i * 4 + 4]);
-      { lemma_seq_suffix_slice(data[start..], 8, i as int * 4, i as int * 4 + 4); }
-      unpack_LittleEndian_Uint32(data[start..][8..][i * 4..i * 4 + 4]);
-      { lemma_seq_extensionality_slice(data[start..][8..], data[start..][8..][..len*4], i as int * 4, i as int * 4 + 4); }
-      unpack_LittleEndian_Uint32(data[start..][8..][..len*4][i * 4..i * 4 + 4]);
-      unpack_LittleEndian_Uint32_Seq(data[start..][8..][0..4*len], len as int)[i];
-      { lemma_seq_suffix_slice(data[start..], 8, 0, 4*len); }
-      unpack_LittleEndian_Uint32_Seq(data[start..][8..8+4*len], len as int)[i];
-      parse_Uint32Array(data[start..]).0.value.va[i];
+      calc {
+        element;
+        unpack_LittleEndian_Uint32(data[start + idx..start + idx + 4]);
+        { lemma_seq_suffix_slice(data, start as int, idx as int, idx as int + 4); }
+        unpack_LittleEndian_Uint32(data[start..][idx..idx + 4]);
+        unpack_LittleEndian_Uint32(data[start..][8 + i * 4..8 + i * 4 + 4]);
+        { lemma_seq_suffix_slice(data[start..], 8, i as int * 4, i as int * 4 + 4); }
+        unpack_LittleEndian_Uint32(data[start..][8..][i * 4..i * 4 + 4]);
+        { lemma_seq_extensionality_slice(data[start..][8..], data[start..][8..][..len*4], i as int * 4, i as int * 4 + 4); }
+        unpack_LittleEndian_Uint32(data[start..][8..][..len*4][i * 4..i * 4 + 4]);
+        unpack_LittleEndian_Uint32_Seq(data[start..][8..][0..4*len], len as int)[i];
+        { lemma_seq_suffix_slice(data[start..], 8, 0, 4*len); }
+        unpack_LittleEndian_Uint32_Seq(data[start..][8..8+4*len], len as int)[i];
+        parse_Uint32Array(data[start..]).0.value.va[i];
+      }
     }
   }
 
